PREFIX : <https://linked.data.gov.au/dataset/bdr/datatypes/>
PREFIX cs: <https://linked.data.gov.au/dataset/bdr/datatypes>
PREFIX rdfs: <http://www.w3.org/2000/01/rdf-schema#>
PREFIX dcat: <http://www.w3.org/ns/dcat#>
PREFIX orgs: <https://linked.data.gov.au/dataset/bdr/orgs/>
PREFIX owl: <http://www.w3.org/2002/07/owl#>
PREFIX schema: <https://schema.org/>
PREFIX skos: <http://www.w3.org/2004/02/skos/core#>
PREFIX xsd: <http://www.w3.org/2001/XMLSchema#>

:WamNumber
    a skos:Concept ;
    a rdfs:Datatype ;
    skos:definition "Western Australian Museum Number - a catalogue number issued by the WA Museum"@en ;
    skos:historyNote "Defined by BDR admin as real datatype expected in data from WA but also as an example" ;
    skos:inScheme cs: ;
    skos:prefLabel "WAM Number"@en ;
    skos:topConceptOf cs: ;
    dcat:contactPoint <https://linked.data.gov.au/org/wam> ;
.

:MERITProjectID
    a skos:Concept ;
    a rdfs:Datatype ;
    skos:definition "String literal type that represents the unique identifier for a Project in MERIT."@en ;
    skos:historyNote "Defined by TERN Australia for use the BDR." ;
    skos:inScheme cs: ;
    skos:prefLabel "MERITProjectID"@en ;
    skos:topConceptOf cs: ;
    dcat:contactPoint <https://linked.data.gov.au/org/tern> ;
.

:MERITCreatorID
    a skos:Concept ;
    a rdfs:Datatype ;
    skos:definition "String literal type that represents the unique identifier for Person in the Creator role of a MERIT submission to the BDR."@en ;
    skos:historyNote "Defined by TERN Australia for use the BDR." ;
    skos:inScheme cs: ;
    skos:prefLabel "MERITCreatorID"@en ;
    skos:topConceptOf cs: ;
    dcat:contactPoint <https://linked.data.gov.au/org/tern> ;
.

cs:
    a skos:ConceptScheme ;
    skos:definition "Literal datatypes defined for use within the Biodiversity Data Repository"@en ;
    skos:hasTopConcept :WamNumber ;
    skos:historyNote "This vocabulary was developed for the Biodiversity Data Repository and is live in that it grows with new data submissions that use define new datatypes" ;
    skos:prefLabel "BDR Datatypes"@en ;
    schema:creator <https://linked.data.gov.au/org/dcceew> ;
    schema:dateCreated "2024-07-09"^^xsd:date ;
    schema:dateModified "2024-12-04"^^xsd:date ;
    schema:license <http://purl.org/NET/rdflicense/cc-by4.0> ;
    schema:publisher <https://linked.data.gov.au/org/dcceew> ;
.
