PREFIX : <https://linked.data.gov.au/dataset/bdr/op/>
PREFIX cs: <https://linked.data.gov.au/dataset/bdr/op>
PREFIX owl: <http://www.w3.org/2002/07/owl#>
PREFIX schema: <https://schema.org/>
PREFIX skos: <http://www.w3.org/2004/02/skos/core#>
PREFIX xsd: <http://www.w3.org/2001/XMLSchema#>


:DataStatistic
    a skos:Concept ;
    skos:definition "A statistic of data within a given scope"@en ;
    skos:historyNote "Defined by BDR admin" ;
    skos:inScheme cs: ;
    skos:prefLabel "Data Statistic"@en ;
    skos:topConceptOf cs: ;
.

:ObservationsCount
    a skos:Concept ;
    skos:definition "The number of ABIS Observation class instances within a given scope"@en ;
    skos:historyNote "Defined by BDR admin" ;
    skos:inScheme cs: ;
    skos:prefLabel "Observations Count"@en ;
    skos:topConceptOf cs: ;
    skos:broader :DataStatistic ;
.

:DatasetsCount
    a skos:Concept ;
    skos:definition "The number of ABIS Dataset class instances within a given scope"@en ;
    skos:historyNote "Defined by BDR admin" ;
    skos:inScheme cs: ;
    skos:prefLabel "Datasets Count"@en ;
    skos:topConceptOf cs: ;
    skos:broader :DataStatistic ;
.

cs:
    a skos:ConceptScheme ;
    skos:definition """Observable properties - things that can be observed - in use in the Biodiversity Data Repository and not elsewhere defined.

These OPs are for anything, e.g. surface texture of a material sample as well as statistics of data."""@en ;
    skos:hasTopConcept :DataStatistic ;
    skos:historyNote "This vocabulary was developed for the Biodiversity Data Repository as a catch-all vocab/register of observable properties which are not characterised elsewhere" ;
    skos:prefLabel "BDR Observable Properties"@en ;
    schema:creator <https://linked.data.gov.au/org/dcceew> ;
    schema:dateCreated "2024-07-10"^^xsd:date ;
    schema:dateModified "2024-07-10"^^xsd:date ;
    schema:license <http://purl.org/NET/rdflicense/cc-by4.0> ;
    schema:publisher <https://linked.data.gov.au/org/dcceew> ;
.
