PREFIX cs: <https://linked.data.gov.au/dataset/bdr/orgs>
PREFIX schema: <https://schema.org/>
PREFIX skos: <http://www.w3.org/2004/02/skos/core#>
PREFIX xsd: <http://www.w3.org/2001/XMLSchema#>

<https://linked.data.gov.au/org/act>
    a
        skos:Concept ,
        schema:Organization ;
    skos:definition "The government of the Australian Capital Territory."@en ;
    skos:inScheme cs: ;
    skos:prefLabel "ACT Government"@en ;
    skos:topConceptOf cs: ;
    schema:name "ACT Government" ;
    schema:url "https://www.act.gov.au"^^xsd:anyURI ;
.

<https://linked.data.gov.au/org/act-atlas>
    a
        skos:Concept ,
        schema:Organization ;
    skos:definition "This spatial dataset maps the location of wildlife records held within the ACT Wildlife Atlas up until December 2014. Records include mammals, fish, amphibians, invertebrates, reptiles and birds."@en ;
    skos:inScheme cs: ;
    skos:prefLabel "ACT Wildlife Atlas"@en ;
    skos:topConceptOf cs: ;
    schema:name "ACT Wildlife Atlas" ;
    schema:url "https://researchdata.edu.au/act-wildlife-atlas/3543262"^^xsd:anyURI ;
.

<https://linked.data.gov.au/org/am>
    a
        skos:Concept ,
        schema:Organization ;
    skos:definition "The Australian Museum is an NSW Government organisation operating under the Department of Creative Industries"@en ;
    skos:inScheme cs: ;
    skos:notation "85 407 224 698"^^<http://id.loc.gov/vocabulary/identifiers/ausbn> ;
    skos:prefLabel "Australian Museum"@en ;
    skos:topConceptOf cs: ;
    schema:name "Australian Museum" ;
    schema:url "https://australian.museum"^^xsd:anyURI ;
.

<https://linked.data.gov.au/org/ambseh>
    a
        skos:Concept ,
        schema:Organization ;
    skos:definition "AMBS Ecology & Heritage is a specialist consultancy providing expert advice and services in Aboriginal and historic heritage and archaeology"@en ;
    skos:inScheme cs: ;
    skos:notation "96 609 155 464"^^<http://id.loc.gov/vocabulary/identifiers/ausbn> ;
    skos:prefLabel "AMBS Ecology & Heritage"@en ;
    skos:topConceptOf cs: ;
    schema:name "AMBS Ecology & Heritage" ;
    schema:url "https://www.ambs.consulting"^^xsd:anyURI ;
.

<https://linked.data.gov.au/org/amnh>
    a
        skos:Concept ,
        schema:Organization ;
    skos:definition """The American Museum of Natural History is one of the world’s preeminent scientific and cultural institutions.

Since its founding in 1869, the Museum has advanced its global mission to discover, interpret, and disseminate information about human cultures, the natural world, and the universe through a wide-ranging program of scientific research, education, and exhibition."""@en ;
    skos:inScheme cs: ;
    skos:prefLabel "American Museum of Natural History"@en ;
    skos:topConceptOf cs: ;
    schema:name "American Museum of Natural History" ;
    schema:url "https://www.amnh.org"^^xsd:anyURI ;
.

<https://linked.data.gov.au/org/ath>
    a
        skos:Concept ,
        schema:Organization ;
    skos:definition "As Australia’s only university established to focus on the issues of Northern Australia and the Tropics worldwide"@en ;
    skos:inScheme cs: ;
    skos:prefLabel "Australian Tropical Herbarium"@en ;
    skos:topConceptOf cs: ;
    schema:name "Australian Tropical Herbarium" ;
    schema:url "https://www.ath.org.au"^^xsd:anyURI ;
.

<https://linked.data.gov.au/org/awc>
    a
        skos:Concept ,
        schema:Organization ;
    skos:definition "Australian Wildlife Conservancy (AWC) protects Australia's unique wildlife through science"@en ;
    skos:inScheme cs: ;
    skos:notation "36 068 572 556"^^<http://id.loc.gov/vocabulary/identifiers/ausbn> ;
    skos:prefLabel "Australian Wildlife Conservancy"@en ;
    skos:topConceptOf cs: ;
    schema:name "Australian Wildlife Conservancy" ;
    schema:url "https://www.australianwildlife.org"^^xsd:anyURI ;
.

<https://linked.data.gov.au/org/awmm>
    a
        skos:Concept ,
        schema:Organization ;
    skos:definition "The Museum is a war memorial for the province of Auckland and holds one of New Zealand's top three heritage libraries. It has pre-eminent Māori and Pacific collections"@en ;
    skos:inScheme cs: ;
    skos:prefLabel "Auckland War Memorial Museum"@en ;
    skos:topConceptOf cs: ;
    schema:name "Auckland War Memorial Museum" ;
    schema:url "https://www.aucklandmuseum.com"^^xsd:anyURI ;
.

<https://linked.data.gov.au/org/baam>
    a
        skos:Concept ,
        schema:Organization ;
    skos:definition "BAAM was established in Brisbane in 2001 to provide terrestrial fauna ecology consulting services. Since that time the company has grown to include botanical expertise, ecological restoration and fauna spotting services. For projects requiring specific expertise we source contribution from within our significant network of ecological specialists to ensure the rigour of our work."@en ;
    skos:inScheme cs: ;
    skos:notation "59 097 464 992"^^<http://id.loc.gov/vocabulary/identifiers/ausbn> ;
    skos:prefLabel "Biodiversity Assessment and Management (BAAM)"@en ;
    skos:topConceptOf cs: ;
    schema:name "Biodiversity Assessment and Management (BAAM)" ;
    schema:url "https://baamecology.com"^^xsd:anyURI ;
.

<https://linked.data.gov.au/org/bdbsa>
    a
        skos:Concept ,
        schema:Organization ;
    skos:definition "The Biological Databases of South Australia (BDBSA) is South Australia's flora and fauna database that stores and manages specimen and observation records"@en ;
    skos:inScheme cs: ;
    skos:prefLabel "Biological Databases of South Australia"@en ;
    skos:topConceptOf cs: ;
    schema:name "Biological Databases of South Australia" ;
    schema:url "https://www.environment.sa.gov.au/topics/science/information-and-data/biological-databases-of-south-australia"^^xsd:anyURI ;
.

<https://linked.data.gov.au/org/bhp>
    a
        skos:Concept ,
        schema:Organization ;
    skos:definition "BHP is a large mining company whose 'purpose is to bring people and resources together to build a better world. We do this through our strategy to deliver long-term value and returns through the cycle.'"@en ;
    skos:inScheme cs: ;
    skos:notation "57 071 987 669"^^<http://id.loc.gov/vocabulary/identifiers/ausbn> ;
    skos:prefLabel "BHP"@en ;
    skos:topConceptOf cs: ;
    schema:name "BHP" ;
    schema:url "https://www.bhp.com"^^xsd:anyURI ;
.

<https://linked.data.gov.au/org/biepa>
    a
        skos:Concept ,
        schema:Organization ;
    skos:definition """BIEPA's mission is to help life to flourish on our island sanctuary by:
* protecting, maintaining, and restoring the native flora and fauna on and around the island;
* monitoring and improving the natural environment, including the surrounding waters;
* influencing urban development and promoting sustainable ecotourism; and
* proactively engaging with the local community to grow our membership and raise funds and awareness."""@en ;
    skos:inScheme cs: ;
    skos:notation "18 064 697 900"^^<http://id.loc.gov/vocabulary/identifiers/ausbn> ;
    skos:prefLabel "Bribie Island Environmental Protection Association Inc"@en ;
    skos:topConceptOf cs: ;
    schema:name "Bribie Island Environmental Protection Association Inc" ;
    schema:url "https://www.biepa.online"^^xsd:anyURI ;
.

<https://linked.data.gov.au/org/birdlife>
    a
        skos:Concept ,
        schema:Organization ;
    skos:definition "Australian Bird science and conservation organisation."@en ;
    skos:historyNote "Added by BDR Admin for the use in the BDR, from AGLDWG Orgs Catalogue https://catalogue.linked.data.gov.au/index.php/org/birdlife" ;
    skos:inScheme cs: ;
    skos:notation "75 149 124 774"^^<http://id.loc.gov/vocabulary/identifiers/ausbn> ;
    skos:prefLabel "BirdLife Australia"@en ;
    skos:topConceptOf cs: ;
    schema:name "BirdLife Australia" ;
    schema:url "https://birdlife.org.au"^^xsd:anyURI ;
.

<https://linked.data.gov.au/org/canbr>
    a
        skos:Concept ,
        schema:Organization ;
    skos:definition "The Centre for Australian National Biodiversity Research (CANBR) includes the Australian National Herbarium. These are jointly managed by CSIRO and the Director of National Parks with strong links to the Australian National Botanic Gardens. The Herbarium"@en ;
    skos:inScheme cs: ;
    skos:prefLabel "Centre for Australian National Biodiversity Research"@en ;
    skos:topConceptOf cs: ;
    schema:name "Centre for Australian National Biodiversity Research" ;
    schema:url "https://www.anbg.gov.au/cpbr"^^xsd:anyURI ;
.

<https://linked.data.gov.au/org/cooloolacc>
    a
        skos:Concept ,
        schema:Organization ;
    skos:definition "Cooloola Coastcare Association is the Cooloola Coast's award winning Natural Resource Management group, registered with Queensland Water and Land Carers (QWALC) and supported by Gympie Regional Council through ratepayer's Environment Levy."@en ;
    skos:inScheme cs: ;
    skos:notation "41 112 645 288"^^<http://id.loc.gov/vocabulary/identifiers/ausbn> ;
    skos:prefLabel "Cooloola Coastcare"@en ;
    skos:topConceptOf cs: ;
    schema:name "Cooloola Coastcare" ;
    schema:url "https://www.cooloolacoastcare.org.au"^^xsd:anyURI ;
.

<https://linked.data.gov.au/org/csiro>
    a
        skos:Concept ,
        schema:Organization ;
    skos:definition "Australia's national science research agency."@en ;
    skos:inScheme cs: ;
    skos:narrower <https://linked.data.gov.au/org/csiro-environment> ;
    skos:notation "41 687 119 230"^^<http://id.loc.gov/vocabulary/identifiers/ausbn> ;
    skos:prefLabel "CSIRO"@en ;
    skos:topConceptOf cs: ;
    schema:name "CSIRO" ;
    schema:url "https://www.csiro.au"^^xsd:anyURI ;
.

<https://linked.data.gov.au/org/csiro-environment>
    a
        skos:Concept ,
        schema:Organization ;
    skos:definition "Australia's national science research agency. Environment Research Unit."@en ;
    skos:inScheme cs: ;
    skos:notation "41 687 119 230"^^<http://id.loc.gov/vocabulary/identifiers/ausbn> ;
    skos:prefLabel "Environment - CSIRO"@en ;
    soks:broader <https://linked.data.gov.au/org/csiro> ;
    schema:name "Environment Research Unit CSIRO" ;
    schema:url "https://www.csiro.au/en/"^^xsd:anyURI ;
.

<https://linked.data.gov.au/org/csiro>
    a
        skos:Concept ,
        schema:Organization ;
    skos:definition "Australia's national science research agency."@en ;
    skos:inScheme cs: ;
    skos:notation "41 687 119 230"^^<http://id.loc.gov/vocabulary/identifiers/ausbn> ;
    skos:prefLabel "CSIRO"@en ;
    skos:topConceptOf cs: ;
    schema:name "CSIRO" ;
    schema:url "https://www.csiro.au"^^xsd:anyURI ;
.

<https://linked.data.gov.au/org/dafwa>
    a
        skos:Concept ,
        schema:Organization ;
    skos:definition "WA Department of Agriculture and Food"@en ;
    skos:inScheme cs: ;
    skos:prefLabel "WA Department of Agriculture and Food"@en ;
    skos:topConceptOf cs: ;
    schema:name "WA Department of Agriculture and Food" ;
    schema:url "https://www.dpird.wa.gov.au"^^xsd:anyURI ;
.

<https://linked.data.gov.au/org/des>
    a
        skos:Concept ,
        schema:Organization ;
    skos:definition "This Department was renamed the Department of Environment, Tourism, Science & Innovation in early 2025."@en ;
    skos:inScheme cs: ;
    skos:prefLabel "Qld Department of Environment and Science"@en ;
    skos:topConceptOf cs: ;
    schema:name "Qld Department of Environment and Science" ;
    schema:url "https://www.detsi.qld.gov.au"^^xsd:anyURI ;
.

<https://linked.data.gov.au/org/ecosmartecology>
    a
        skos:Concept ,
        schema:Organization ;
    skos:definition "EcoSmart Ecology is an emerging industry leader in ecological research, survey and assessment with a strong client focus and the highest commitment to quality. Use our balance of knowledge, skills and experience to assist in navigating through the array of environmental issues and statutory requirements facing ecological planners and developers."@en ;
    skos:inScheme cs: ;
    skos:notation "34 137 963 190"^^<http://id.loc.gov/vocabulary/identifiers/ausbn> ;
    skos:prefLabel "EcoSmart Ecology"@en ;
    skos:topConceptOf cs: ;
    schema:name "EcoSmart Ecology" ;
    schema:url "https://ecosmartecology.com.au"^^xsd:anyURI ;
.

<https://linked.data.gov.au/org/gaia-resources>
    a
        skos:Concept ,
        schema:Organization ;
    skos:definition "Gaia Resources provides a range of services around technology consulting to organisations that work with the environment"@en ;
    skos:inScheme cs: ;
    skos:notation "94 119 508 824"^^<http://id.loc.gov/vocabulary/identifiers/ausbn> ;
    skos:prefLabel "Gaia Resources"@en ;
    skos:topConceptOf cs: ;
    schema:name "Gaia Resources" ;
    schema:url "https://www.gaiaresources.com.au"^^xsd:anyURI ;
.

<https://linked.data.gov.au/org/gccc>
    a
        skos:Concept ,
        schema:Organization ;
    skos:definition "The council of the Gold Coast"@en ;
    skos:inScheme cs: ;
    skos:notation "84 858 548 460"^^<http://id.loc.gov/vocabulary/identifiers/ausbn> ;
    skos:prefLabel "Gold Coast City Council"@en ;
    skos:topConceptOf cs: ;
    schema:name "Gold Coast City Council" ;
    schema:url "https://www.goldcoast.qld.gov.au"^^xsd:anyURI ;
.

<https://linked.data.gov.au/org/jcu>
    a
        skos:Concept ,
        schema:Organization ;
    skos:definition "James Cook University (JCU) is a public university in North Queensland, Australia. The second oldest university in Queensland, JCU is a teaching and research institution. The university's main campuses are located in the tropical cities of Cairns and Townsville, and one in the city state of Singapore. JCU also has study centres in Mount Isa, Mackay, Thursday Island and Rockhampton."@en ;
    skos:inScheme cs: ;
    skos:notation "46 253 211 955"^^<http://id.loc.gov/vocabulary/identifiers/ausbn> ;
    skos:prefLabel "James Cook University"@en ;
    skos:topConceptOf cs: ;
    schema:name "James Cook University" ;
    schema:url "https://www.jcu.edu.au"^^xsd:anyURI ;
.

<https://linked.data.gov.au/org/latrobe>
    a
        skos:Concept ,
        schema:Organization ;
    skos:definition "La Trobe University is a public research university based in Melbourne"@en ;
    skos:inScheme cs: ;
    skos:notation "64 804 735 113"^^<http://id.loc.gov/vocabulary/identifiers/ausbn> ;
    skos:prefLabel "La Trobe University"@en ;
    skos:topConceptOf cs: ;
    schema:name "La Trobe University" ;
    schema:url "https://www.latrobe.edu.au"^^xsd:anyURI ;
.

<https://linked.data.gov.au/org/lcai>
    a
        skos:Concept ,
        schema:Organization ;
    skos:definition "Organisation found in ABR but not online"@en ;
    skos:inScheme cs: ;
    skos:notation "56 756 200 363"^^<http://id.loc.gov/vocabulary/identifiers/ausbn> ;
    skos:prefLabel "Lockyer Catchment Association Inc"@en ;
    skos:topConceptOf cs: ;
    schema:name "Lockyer Catchment Association Inc" ;
    schema:url "https://abr.business.gov.au/ABN/View?abn=56756200363"^^xsd:anyURI ;
.

<https://linked.data.gov.au/org/macleaymuseum>
    a
        skos:Concept ,
        schema:Organization ;
    skos:definition "This museum was formerly part of the University of Sydney but it has been abolished now and its contents transfered to the chau Chack Wing museum within the university."@en ;
    skos:inScheme cs: ;
    skos:prefLabel "Macleay Museum"@en ;
    skos:topConceptOf cs: ;
    schema:name "Macleay Museum" ;
    schema:url "https://en.wikipedia.org/wiki/Macleay_Museum"^^xsd:anyURI ;
.

<https://linked.data.gov.au/org/mboca>
    a
        skos:Concept ,
        schema:Organization ;
    skos:definition "Now part of BirdLife Australia"@en ;
    skos:inScheme cs: ;
    skos:prefLabel "Mackay Bird Observers Club of Australia"@en ;
    skos:topConceptOf cs: ;
    schema:name "Mackay Bird Observers Club of Australia" ;
    schema:url "https://en.wikipedia.org/wiki/Bird_Observation_%26_Conservation_Australia"^^xsd:anyURI ;
.

<https://linked.data.gov.au/org/mgrt>
    a
        skos:Concept ,
        schema:Organization ;
    skos:definition "The Mahogany Glider Recovery Team (MGRT) provides advice and coordinates actions identified in the Mahogany Glider Recovery Plan. The MGRT includes representatives from organisations with a direct interest in the recovery of the Mahogany Glider, including those involved in funding and those participating in actions that support the recovery of the species."@en ;
    skos:inScheme cs: ;
    skos:prefLabel "Mahogany Glider Recovery Team"@en ;
    skos:topConceptOf cs: ;
    schema:name "Mahogany Glider Recovery Team" ;
    schema:url "https://www.wettropicsplan.org.au/contacts-plan-partners/mahogany-glider-recovery-team"^^xsd:anyURI ;
.

<https://linked.data.gov.au/org/mjdenv>
    a
        skos:Concept ,
        schema:Organization ;
    skos:definition "MJD Environmental is an innovative Environmental Consultancy local to the Hunter and servicing the Hunter Valley and beyond in the Land Development"@en ;
    skos:inScheme cs: ;
    skos:notation "58 609 765 693"^^<http://id.loc.gov/vocabulary/identifiers/ausbn> ;
    skos:prefLabel "MJD Environmental"@en ;
    skos:topConceptOf cs: ;
    schema:name "MJD Environmental" ;
    schema:url "https://www.mjdenvironmental.com"^^xsd:anyURI ;
.

<https://linked.data.gov.au/org/mrcca>
    a
        skos:Concept ,
        schema:Organization ;
    skos:definition "The Mary River Catchment Coordination Association is a very active Integrated Catchment Management organisation overseen by the Mary River Catchment Coordinating Committee (MRCCC), which comprises interest sector representatives from 30 community, industry and government sectors with interests in sustainable natural resource management. Today the group reaches out to thousands of catchment residents through our stakeholder delegates and associated networks throughout the catchment."@en ;
    skos:inScheme cs: ;
    skos:notation "23 009 920 786 "^^<http://id.loc.gov/vocabulary/identifiers/ausbn> ;
    skos:prefLabel "Mary River Catchment Coordination Association"@en ;
    skos:topConceptOf cs: ;
    schema:name "Mary River Catchment Coordination Association" ;
    schema:url "https://mrccc.org.au"^^xsd:anyURI ;
.

<https://linked.data.gov.au/org/museumsvictoria>
    a
        skos:Concept ,
        schema:Organization ;
    skos:definition """For more than 160 years, the people of Victoria have turned to their State museum to connect the past and the present, and to imagine the future. As Australia's largest public museum organisation, we inspire audiences to engage in life’s deep mysteries and big questions.

Our museums present unique and exceptional experiences for more than 2 million visitors each year, who come from all over Australia and around the world to be inspired and to learn about themselves and the universe we inhabit.

The collection is an invaluable record of Victoria's environmental and cultural history, and our amazing wealth of over 15 million items has been creating a sense of wonder and awe in visitors for generations."""@en ;
    skos:inScheme cs: ;
    skos:notation "63 640 679 155"^^<http://id.loc.gov/vocabulary/identifiers/ausbn> ;
    skos:prefLabel "Museums Victoria"@en ;
    skos:topConceptOf cs: ;
    schema:name "Museums Victoria" ;
    schema:url "https://museumsvictoria.com.au"^^xsd:anyURI ;
.

<https://linked.data.gov.au/org/mwlr>
    a
        skos:Concept ,
        schema:Organization ;
    skos:definition "Manaaki Whenua – Landcare Research is one of seven Crown Research Institutes (CRIs) formed in 1992. CRIs function as independent companies but are owned by"@en ;
    skos:inScheme cs: ;
    skos:prefLabel "Manaaki Whenua – Landcare Research"@en ;
    skos:topConceptOf cs: ;
    schema:name "Manaaki Whenua – Landcare Research" ;
    schema:url "https://www.landcareresearch.co.nz"^^xsd:anyURI ;
.

<https://linked.data.gov.au/org/naturemapr>
    a
        skos:Concept ,
        schema:Organization ;
    skos:definition "NatureMapr empowers decision makers through citizen-supplied biodiversity data"@en ;
    skos:inScheme cs: ;
    skos:notation "75 119 895 703"^^<http://id.loc.gov/vocabulary/identifiers/ausbn> ;
    skos:prefLabel "Canberra and National NatureMapr Network Incorporated"@en ;
    skos:topConceptOf cs: ;
    schema:name "Canberra and National NatureMapr Network Incorporated" ;
    schema:url "https://canberra.naturemapr.org"^^xsd:anyURI ;
.

<https://linked.data.gov.au/org/nhm>
    a
        skos:Concept ,
        schema:Organization ;
    skos:definition """The Natural History Museum is a world-class visitor attraction and leading science research centre.

We use our unique collections and unrivalled expertise to tackle the biggest challenges facing the world today.

We care for more than 80 million objects spanning billions of years and welcome more than five million visitors annually."""@en ;
    skos:inScheme cs: ;
    skos:prefLabel "Natural History Museum"@en ;
    skos:topConceptOf cs: ;
    schema:name "Natural History Museum" ;
    schema:url "https://www.nhm.ac.uk"^^xsd:anyURI ;
.

<https://linked.data.gov.au/org/npansw>
    a
        skos:Concept ,
        schema:Organization ;
    skos:definition """The National Parks Association of NSW (commonly known as NPA) is a member-based conservation organisation and registered charity. Our mission is protecting nature through community action.

We are committed to protecting, conserving and restoring the integrity and diversity of nature, its biodiversity, geodiversity, supporting ecological processes and associated cultural values. We complement our conservation work by providing rewarding and enjoyable opportunities for people to experience, appreciate, study and care for nature."""@en ;
    skos:inScheme cs: ;
    skos:notation "67 694 961 955"^^<http://id.loc.gov/vocabulary/identifiers/ausbn> ;
    skos:prefLabel "NPANSW"@en ;
    skos:topConceptOf cs: ;
    schema:name "NPANSW" ;
    schema:url "https://npansw.org.au"^^xsd:anyURI ;
.

<https://linked.data.gov.au/org/nsw-bionet>
    a
        skos:Concept ,
        schema:Organization ;
    skos:definition "The gateway to NSW biodiversity information."@en ;
    skos:inScheme cs: ;
    skos:prefLabel "NSW BioNet"@en ;
    skos:topConceptOf cs: ;
    schema:name "NSW BioNet" ;
    schema:url "https://www.environment.nsw.gov.au/topics/animals-and-plants/biodiversity/nsw-bionet"^^xsd:anyURI ;
.

<https://linked.data.gov.au/org/nsw-daff>
    a
        skos:Concept ,
        schema:Organization ;
    skos:definition "From 1 July 2024, the NSW Department of Primary Industries Forests became part of the newly formed NSW Department of Primary Industries and Regional Development."@en ;
    skos:inScheme cs: ;
    skos:prefLabel "NSW Department of Primary Industries Forests"@en ;
    skos:topConceptOf cs: ;
    schema:name "NSW Department of Primary Industries Forests" ;
    schema:url "https://www.dpi.nsw.gov.au/forestry"^^xsd:anyURI ;
.

<https://linked.data.gov.au/org/nsw-dcceew>
    a
        skos:Concept ,
        schema:Organization ;
    skos:definition "The NSW Department of Climate Change, Energy, the Environment and Water (DCCEEW) works to protect the state’s environment and heritage. It leads the way on climate change, driving the sustainable transition to a net zero economy, powered by affordable, reliable, and clean energy."@en ;
    skos:inScheme cs: ;
    skos:notation "27 578 976 844"^^<http://id.loc.gov/vocabulary/identifiers/ausbn> ;
    skos:prefLabel "NSW Department of Climate Change, Energy, the Environment and Water"@en ;
    skos:topConceptOf cs: ;
    schema:name "NSW Department of Climate Change, Energy, the Environment and Water" ;
    schema:url "https://www.nsw.gov.au/departments-and-agencies/dcceew"^^xsd:anyURI ;
.

<https://linked.data.gov.au/org/nsw-dpe>
    a
        skos:Concept ,
        schema:Organization ;
    skos:definition """The New South Wales Department of Planning and Environment (DPE) was a department of the New South Wales Government, responsible for effective and sustainable planning to support the growth in the state of New South Wales, Australia.

The department was renamed from the Department of Planning, Industry and Environment (DPIE) on 21 December 2021.

Superseding agencies: Department of Planning, Housing and Infrastructure & Department of Climate Change, Energy, the Environment and Water."""@en ;
    skos:inScheme cs: ;
    skos:prefLabel "NSW Dept of Planning and Environment"@en ;
    skos:topConceptOf cs: ;
    schema:name "NSW Dept of Planning and Environment" ;
    schema:url "https://www.dpie.nsw.gov.au"^^xsd:anyURI ;
.

<https://linked.data.gov.au/org/nsw-dpie>
    a
        skos:Concept ,
        schema:Organization ;
    skos:definition "The New South Wales Department of Department of Planning, Industry and Environment (DPIE) was renamed to the Department of Planning and Environment (DPE) on 21 December 2021."@en ;
    skos:inScheme cs: ;
    skos:prefLabel "NSW Dept of Planning Industry and Environment"@en ;
    skos:topConceptOf cs: ;
    schema:name "NSW Dept of Planning Industry and Environment" ;
    schema:url "https://www.dpie.nsw.gov.au"^^xsd:anyURI ;
.

<https://linked.data.gov.au/org/nsw-npws>
    a
        skos:Concept ,
        schema:Organization ;
    skos:definition "NSW National Parks and Wildlife Service (NPWS) is part of Environment and Heritage in the Department of Climate Change"@en ;
    skos:inScheme cs: ;
    skos:notation "27 578 976 844"^^<http://id.loc.gov/vocabulary/identifiers/ausbn> ;
    skos:prefLabel "NSW National Parks and Wildlife Service"@en ;
    skos:topConceptOf cs: ;
    schema:name "NSW National Parks and Wildlife Service" ;
    schema:url "https://www.nationalparks.nsw.gov.au"^^xsd:anyURI ;
.

<https://linked.data.gov.au/org/nt-atlas>
    a
        skos:Concept ,
        schema:Organization ;
    skos:definition "This is a comprehensive database of all known vertebrate fauna records, including mammals, birds, reptiles, frogs and fish, as well threatened invertebrates, for the Northern Territory."@en ;
    skos:inScheme cs: ;
    skos:prefLabel "NT Fauna Atlas"@en ;
    skos:topConceptOf cs: ;
    schema:name "NT Fauna Atlas" ;
    schema:url "https://data.nt.gov.au/dataset/nt-fauna-atlas"^^xsd:anyURI ;
.

<https://linked.data.gov.au/org/nt-dipe>
    a
        skos:Concept ,
        schema:Organization ;
    skos:definition "The Northern Territory Department of Infrastructure, Planning and Environment is now called the Department of Logistics and Infrastructure (DLI). It was previously named the Department of Infrastructure, Planning and Logistics (DIPL). The DLI was established in September 2024 by the Northern Territory Government. It focuses on infrastructure, logistics, and sustainable development across the Northern Territory."@en ;
    skos:inScheme cs: ;
    skos:prefLabel "Northern Territory Department of Infrastructure, Planning and Environment"@en ;
    skos:topConceptOf cs: ;
    schema:name "Northern Territory Department of Infrastructure, Planning and Environment" ;
    schema:url "https://environment.nt.gov.au"^^xsd:anyURI ;
.

<https://linked.data.gov.au/org/nt-dlpe>
    a
        skos:Concept ,
        schema:Organization ;
    skos:definition "The department includes the key functions that foster and protect the environment and natural resources in the Northern Territory."@en ;
    skos:inScheme cs: ;
    skos:notation "84 085 734 992"^^<http://id.loc.gov/vocabulary/identifiers/ausbn> ;
    skos:prefLabel "NT Department of Lands Planning and Environment"@en ;
    skos:topConceptOf cs: ;
    schema:name "NT Department of Lands Planning and Environment" ;
    schema:url "https://environment.nt.gov.au"^^xsd:anyURI ;
.

<https://linked.data.gov.au/org/nt-dlrm>
    a
        skos:Concept ,
        schema:Organization ;
    skos:definition "The Department has been superseded by the Department of Lands"@en ;
    skos:inScheme cs: ;
    skos:prefLabel "NT Department of Land Resource Management"@en ;
    skos:topConceptOf cs: ;
    schema:name "NT Department of Land Resource Management" ;
    schema:url "https://environment.nt.gov.au"^^xsd:anyURI ;
.

<https://linked.data.gov.au/org/nt-herbarium>
    a
        skos:Concept ,
        schema:Organization ;
    skos:definition """A herbarium is a 'museum or library of plant specimens'. They are part of an international network dedicated to the study and identification of plants.

The NT Herbarium has a collection of 270,000 preserved plant specimens kept for reference and research."""@en ;
    skos:inScheme cs: ;
    skos:prefLabel "NT Herbarium"@en ;
    skos:topConceptOf cs: ;
    schema:name "NT Herbarium" ;
    schema:url "https://nt.gov.au/environment/native-plants/native-plants-and-nt-herbarium"^^xsd:anyURI ;
.

<https://linked.data.gov.au/org/qld-daff>
    a
        skos:Concept ,
        schema:Organization ;
    skos:definition
        """The Department of Agriculture and Fisheries (DAF) was officially dissolved and replaced by the Department of Primary Industries (DPI) on 1 November 2024, due to machinery of government changes.

Formerly known as the Department of Agriculture and Fisheries.

We ensure that Queensland’s primary industries—the essential backbone of our economy and communities—are productive, profitable and sustainable for future generations.

We do this by connecting industries, the community and government to grow our economy, protect our primary industries from biosecurity threats and support rural communities."""@en ;
    skos:inScheme cs: ;
    skos:notation "66 934 348 189"^^<http://id.loc.gov/vocabulary/identifiers/ausbn> ;
    skos:prefLabel "Qld Department of Agriculture and Fisheries"@en ;
    skos:topConceptOf cs: ;
    schema:name "Qld Department of Agriculture and Fisheries" ;
    schema:url
        "https://www.archivessearch.qld.gov.au/agencies/A11656"^^xsd:anyURI ;
.

<https://linked.data.gov.au/org/qld-derm>
    a
        skos:Concept ,
        schema:Organization ;
    skos:definition "DERM was dissolved and transformed into the Department of Environment and Heritage Protection (EHP) in 2012"@en ;
    skos:inScheme cs: ;
    skos:prefLabel "Qld Department of Environment and Resource Management"@en ;
    skos:topConceptOf cs: ;
    schema:name "Qld Department of Environment and Resource Management" ;
    schema:url "https://www.archivessearch.qld.gov.au/agencies/A11171"^^xsd:anyURI ;
.

<https://linked.data.gov.au/org/qld-detsi>
    a
        skos:Concept ,
        schema:Organization ;
    skos:definition """Our department recognises the enormous value a clean environment, innovative society and visitor economy, and vibrant culture contributes to our lives.

As a diverse organisation, the department brings together key areas of work to achieve our objectives for a better Queensland."""@en ;
    skos:inScheme cs: ;
    skos:notation "46 640 294 485"^^<http://id.loc.gov/vocabulary/identifiers/ausbn> ;
    skos:prefLabel "Department of Environment Tourism Science and Innovation"@en ;
    skos:topConceptOf cs: ;
    schema:name "Department of Environment Tourism Science and Innovation" ;
    schema:url "https://www.detsi.qld.gov.au"^^xsd:anyURI ;
.

<https://linked.data.gov.au/org/qld-dres>
    a
        skos:Concept ,
        schema:Organization ;
    skos:definition "The Department of Resources was renamed the Department of Natural Resources and Mines, Manufacturing and Regional and Rural Development in 2025"@en ;
    skos:inScheme cs: ;
    skos:prefLabel "Qld Department of Resources"@en ;
    skos:topConceptOf cs: ;
    schema:name "Qld Department of Resources" ;
    schema:url "https://www.resources.qld.gov.au"^^xsd:anyURI ;
.

<https://linked.data.gov.au/org/qld-tmr>
    a
        skos:Concept ,
        schema:Organization ;
    skos:definition """The Department of Transport and Main Roads moves and connects people, places, goods and services safely, efficiently and effectively across Queensland.
We plan, manage and deliver Queensland's integrated transport environment to achieve sustainable transport solutions for road, rail, air and sea."""@en ;
    skos:inScheme cs: ;
    skos:notation "39 407 690 291"^^<http://id.loc.gov/vocabulary/identifiers/ausbn> ;
    skos:prefLabel "Qld Department of Transport and Main Roads"@en ;
    skos:topConceptOf cs: ;
    schema:name "Qld Department of Transport and Main Roads" ;
    schema:url "https://www.tmr.qld.gov.au"^^xsd:anyURI ;
.

<https://linked.data.gov.au/org/qld-tsgehp>
    a
        skos:Concept ,
        schema:Organization ;
    skos:definition "Part of Department of the Environment, Tourism, Science and Innovation (DETSI)"@en ;
    skos:inScheme cs: ;
    skos:prefLabel "Qld Threatened Species Group"@en ;
    skos:topConceptOf cs: ;
    schema:name "Qld Threatened Species Group" ;
    schema:url "https://www.detsi.qld.gov.au"^^xsd:anyURI ;
.

<https://linked.data.gov.au/org/qld-wildnet>
    a
        skos:Concept ,
        schema:Organization ;
    skos:definition "WildNet is home to wildlife sightings, survey results, species profiles and multimedia."@en ;
    skos:inScheme cs: ;
    skos:prefLabel "WildNet platform"@en ;
    skos:topConceptOf cs: ;
    schema:name "WildNet platform" ;
    schema:url "https://www.qld.gov.au/environment/plants-animals/species-information/wildnet"^^xsd:anyURI ;
.

<https://linked.data.gov.au/org/qm>
    a
        skos:Concept ,
        schema:Organization ;
    skos:definition "Queensland Museum is the keeping place for the State Collection, a magnificent assemblage of 1.2 million cultural objects, natural history specimens and geological treasures and more than 14 million research items. Every year, we bring our collections to life through fieldwork, contemporary acquisitions, world-class research and a dynamic program of exhibitions, workshops, talks, lectures and major events including World Science Festival Brisbane."@en ;
    skos:inScheme cs: ;
    skos:notation "91 522 611 802"^^<http://id.loc.gov/vocabulary/identifiers/ausbn> ;
    skos:prefLabel "Queensland Museum"@en ;
    skos:topConceptOf cs: ;
    schema:name "Queensland Museum" ;
    schema:url "https://www.museum.qld.gov.au"^^xsd:anyURI ;
.

<https://linked.data.gov.au/org/qnc>
    a
        skos:Concept ,
        schema:Organization ;
    skos:definition "The Queensland Naturalists’ Club Inc aims to study all branches of natural history, to encourage the preservation and protection of native flora and fauna and their environments. We also focus on publishing worthwhile observations on natural history and record club activities."@en ;
    skos:inScheme cs: ;
    skos:notation "22 586 275 203"^^<http://id.loc.gov/vocabulary/identifiers/ausbn> ;
    skos:prefLabel "Queensland-Naturalists-Club"@en ;
    skos:topConceptOf cs: ;
    schema:name "Queensland-Naturalists-Club" ;
    schema:url "https://www.qnc.org.au"^^xsd:anyURI ;
.

<https://linked.data.gov.au/org/qpws>
    a
        skos:Concept ,
        schema:Organization ;
    skos:definition "Part of Qld DETSI"@en ;
    skos:inScheme cs: ;
    skos:prefLabel "Queensland Parks and Wildlife Service"@en ;
    skos:topConceptOf cs: ;
    schema:name "Queensland Parks and Wildlife Service" ;
    schema:url "https://parks.desi.qld.gov.au"^^xsd:anyURI ;
.

<https://linked.data.gov.au/org/qvmag>
    a
        skos:Concept ,
        schema:Organization ;
    skos:definition "The Queen Victoria Museum and Art Gallery (QVMAG) is the cultural hub of Launceston and the leading destination for art, history and natural sciences in Northern Tasmania. "@en ;
    skos:inScheme cs: ;
    skos:notation "73 149 070 625"^^<http://id.loc.gov/vocabulary/identifiers/ausbn> ;
    skos:prefLabel "Queen Victoria Museum & Art Gallery"@en ;
    skos:topConceptOf cs: ;
    schema:name "Queen Victoria Museum & Art Gallery" ;
    schema:url "https://www.qvmag.tas.gov.au"^^xsd:anyURI ;
.

<https://linked.data.gov.au/org/rbgdt>
    a
        skos:Concept ,
        schema:Organization ;
    skos:definition """Botanic Gardens of Sydney encompasses three world-leading botanic gardens, Australia’s premier botanical research institute, and Sydney’s leading outdoor activation precinct.

As Australia’s oldest scientific institution, we are custodians of more than $1.2 billion in state significant cultural, heritage and botanical collections.

The Gardens are a leading entity within the tourism sector with a focus on engaging international, national and regional visitors.

Botanic Gardens of Sydney is the registered business name of the Royal Botanic Gardens and Domain Trust, which is constituted under the Royal Botanic Gardens and Domain Trust Act 1980."""@en ;
    skos:inScheme cs: ;
    skos:prefLabel "Royal Botanic Gardens and Domain Trust"@en ;
    skos:topConceptOf cs: ;
    schema:name "Royal Botanic Gardens and Domain Trust" ;
    schema:url "https://www.service.nsw.gov.au/nswgovdirectory/royal-botanic-gardens-and-domain-trust-the"^^xsd:anyURI ;
.

<https://linked.data.gov.au/org/rbgv>
    a
        skos:Concept ,
        schema:Organization ;
    skos:definition """Royal Botanic Gardens Victoria plays a leading role in the conservation of plants through biodiversity research, programs to protect rare and threatened plants, and the study of habitats. This work is supported by education and visitor programs about the importance of plants to life.

The organisation encompasses two diverse sites at Melbourne and Cranbourne and the State Botanical Collection housed at the National Herbarium of Victoria. Royal Botanic Gardens Victoria is managed by the Royal Botanic Gardens Board Victoria, which is responsible to the Minister for Environment."""@en ;
    skos:inScheme cs: ;
    skos:prefLabel "Royal Botanic Gardens Victoria"@en ;
    skos:topConceptOf cs: ;
    schema:name "Royal Botanic Gardens Victoria" ;
    schema:url "https://www.rbg.vic.gov.au"^^xsd:anyURI ;
.

<https://linked.data.gov.au/org/reefcatchments>
    a
        skos:Concept ,
        schema:Organization ;
    skos:definition "Reef Catchments is the Natural Resource Management (NRM) organisation for the Mackay Whitsunday Isaac region. We facilitate change and work for long-term solutions to sustain, protect, and improve our region’s natural resources and environment, both now and into the future."@en ;
    skos:inScheme cs: ;
    skos:notation "26 873 357 348"^^<http://id.loc.gov/vocabulary/identifiers/ausbn> ;
    skos:prefLabel "Reef Catchments"@en ;
    skos:topConceptOf cs: ;
    schema:name "Reef Catchments" ;
    schema:url "https://reefcatchments.com.au"^^xsd:anyURI ;
.

<https://linked.data.gov.au/org/riotinto>
    a
        skos:Concept ,
        schema:Organization ;
    skos:definition "Rio Tinto Group is a British-Australian multinational company that is the world's second largest metals and mining corporation."@en ;
    skos:inScheme cs: ;
    skos:notation "96 004 458 404"^^<http://id.loc.gov/vocabulary/identifiers/ausbn> ;
    skos:prefLabel "Rio Tinto"@en ;
    skos:topConceptOf cs: ;
    schema:name "Rio Tinto" ;
    schema:url "https://www.riotinto.com"^^xsd:anyURI ;
.

<https://linked.data.gov.au/org/sa-dew>
    a
        skos:Concept ,
        schema:Organization ;
    skos:definition "The Department for Environment and Water (DEW) manages a complex portfolio of natural and built assets that are critical to the wellbeing and economic prosperity of all South Australians."@en ;
    skos:inScheme cs: ;
    skos:prefLabel "SA Department for Environment and Water"@en ;
    skos:topConceptOf cs: ;
    schema:name "SA Department for Environment and Water" ;
    schema:url "https://www.environment.sa.gov.au"^^xsd:anyURI ;
.

<https://linked.data.gov.au/org/sa-dewnr>
    a
        skos:Concept ,
        schema:Organization ;
    skos:definition "The South Australian Department for Environment, Water and Natural Resources (DEWNR) has changed its name. It is now the Department for Environment and Water (DEW). This name change occurred on March 22, 2018, according to State Records South Australia. The change was due to adjustments in ministerial portfolios and reporting lines. "@en ;
    skos:inScheme cs: ;
    skos:notation "36 702 093 234"^^<http://id.loc.gov/vocabulary/identifiers/ausbn> ;
    skos:prefLabel "SA Department for Environment and Water"@en ;
    skos:topConceptOf cs: ;
    schema:name "SA Department for Environment and Water" ;
    schema:url "https://www.environment.sa.gov.au"^^xsd:anyURI ;
.

<https://linked.data.gov.au/org/sa-herbarium>
    a
        skos:Concept ,
        schema:Organization ;
    skos:definition """The State Herbarium of South Australia, sometimes called the South Australian Herbarium, and having the herbarium code, AD, is located in Adelaide, South Australia. It is one of several State and Commonwealth herbaria in Australia. The Department for Environment and Water is the state agency which is responsible for the Herbarium, but the Board of the Botanic Gardens and State Herbarium (established by an Act of Parliament, most recently the Botanic Gardens and State Herbarium Act 1978) is charged with its establishment and maintenance.

The herbarium is responsible for Electronic Flora of South Australia. It also produces the journal, Swainsona (formerly Journal of the Adelaide Botanic Gardens)."""@en ;
    skos:inScheme cs: ;
    skos:prefLabel "State Herbarium of South Australia"@en ;
    skos:topConceptOf cs: ;
    schema:name "State Herbarium of South Australia" ;
    schema:url "https://www.botanicgardens.sa.gov.au/science/research/state-herbarium"^^xsd:anyURI ;
.

<https://linked.data.gov.au/org/sam>
    a
        skos:Concept ,
        schema:Organization ;
    skos:definition "The South Australian Museum has been committed to making Australia’s natural and cultural heritage accessible, engaging and fun for over 165 years. It is a place where families can learn and grow together. Today the Museum is one of the most visited museums in Australia and holds collections of national and international significance. It is a leader in remote and regional community engagement, and in Australian Aboriginal heritage and scientific research."@en ;
    skos:inScheme cs: ;
    skos:notation "39 808 959 302"^^<http://id.loc.gov/vocabulary/identifiers/ausbn> ;
    skos:prefLabel "South Australian Museum"@en ;
    skos:topConceptOf cs: ;
    schema:name "South Australian Museum" ;
    schema:url "https://www.samuseum.sa.gov.au"^^xsd:anyURI ;
.

<https://linked.data.gov.au/org/scienceforwildlife>
    a
        skos:Concept ,
        schema:Organization ;
    skos:definition """Science for Wildlife is a leading not-for-profit conservation organisation working to ensure a future for wildlife and the places they call home.

Bringing the best available science to wildlife conservation in Australia and beyond, through the creation and sharing of ecological knowledge we empower people to participate in conservation that has an on-the-ground, enduring impact. Working with iconic and important species in key areas, our research and conservation work is designed to bring broader ecosystem benefits, maximising gains for many other animals and their habitats. We work beyond fences, at a landscape scale to bring real world solutions to conservation challenges. Our work is highly regarded by government and industry partners and informs conservation policy and action both nationally and globally."""@en ;
    skos:inScheme cs: ;
    skos:prefLabel "Science for Wildlife"@en ;
    skos:topConceptOf cs: ;
    schema:name "Science for Wildlife" ;
    schema:url "https://www.scienceforwildlife.org"^^xsd:anyURI ;
.

<https://linked.data.gov.au/org/scion>
    a
        skos:Concept ,
        schema:Organization ;
    skos:definition "Scion is a group of the New Zealand Institute for Bioeconomy Science"@en ;
    skos:inScheme cs: ;
    skos:prefLabel "Scion Crown Research Institute of NZ"@en ;
    skos:topConceptOf cs: ;
    schema:name "Scion Crown Research Institute of NZ" ;
    schema:url "https://www.scionresearch.com"^^xsd:anyURI ;
.

<https://linked.data.gov.au/org/sfsgi>
    a
        skos:Concept ,
        schema:Organization ;
    skos:definition """The Sydney Fungal Studies Group Incorporated (SFSGI) consists of mycological and other academics, students, and many other, non-academic but interested people of all age groups.

The SFSGI aims to advance the study of fungi at all levels, particularly the larger fungi, to educate people at all stages of skill and knowledge in the science of mycology, and to interact with groups and societies having mycological or closely related interests.

Membership is open to all, with the only requirements being that they are interested in contributing to the activities of the Group, subscribe to the aims of the Group, and that they respect the basic principles of nature conservation."""@en ;
    skos:inScheme cs: ;
    skos:notation "76 384 308 862"^^<http://id.loc.gov/vocabulary/identifiers/ausbn> ;
    skos:prefLabel "Sydney Fungal Studies Group"@en ;
    skos:topConceptOf cs: ;
    schema:name "Sydney Fungal Studies Group" ;
    schema:url "https://www.sydneyfungalstudies.org.au"^^xsd:anyURI ;
.

<https://linked.data.gov.au/org/sunwater>
    a
        skos:Concept ,
        schema:Organization ;
    skos:definition "Sunwater is a Queensland-based water service provider, making the most of the available water supply for our agriculture, urban and industrial customers."@en ;
    skos:inScheme cs: ;
    skos:notation "17 020 276 523"^^<http://id.loc.gov/vocabulary/identifiers/ausbn> ;
    skos:prefLabel "SunWater"@en ;
    skos:topConceptOf cs: ;
    schema:name "SunWater" ;
    schema:url "https://www.sunwater.com.au"^^xsd:anyURI ;
.

<https://linked.data.gov.au/org/tas-nre>
    a
        skos:Concept ,
        schema:Organization ;
    skos:definition """The Department of Natural Resources and Environment Tasmania (NRE Tas) is responsible for delivering a sustainable Tasmania. 
We deliver a sustainable Tasmania by protecting and enhancing Tasmania's cultural and natural values; facilitating productive and sustainable industries; and by promoting the sustainable use, presentation, and enjoyment of our cultural and natural values."""@en ;
    skos:inScheme cs: ;
    skos:prefLabel "Department of Natural Resources and Environment Tasmania"@en ;
    skos:altLabel "NRE Tas" ;
    skos:topConceptOf cs: ;
    schema:name "Department of Natural Resources and Environment Tasmania" ;
    schema:url "https://www.nre.tas.gov.au"^^xsd:anyURI ;
.

<https://linked.data.gov.au/org/tas-nva>
    a
        skos:Concept ,
        schema:Organization ;
    skos:definition "The Natural Values Atlas provides authoritative and comprehensive information on Tasmania's natural values."@en ;
    skos:inScheme cs: ;
    skos:prefLabel "Tasmanian Natural Values Atlas"@en ;
    skos:altLabel "NVA" ;
    skos:topConceptOf cs: ;
    schema:name "Tasmanian Natural Values Atlas" ;
    schema:url "https://www.naturalvaluesatlas.tas.gov.au"^^xsd:anyURI ;
.

<https://linked.data.gov.au/org/te-papa>
    a
        skos:Concept ,
        schema:Organization ;
    skos:definition "Te Papa is New Zealand's national museum, renowned for being bicultural, scholarly, innovative, and fun. Our success is built on our relationships with and our ability to represent our community."@en ;
    skos:inScheme cs: ;
    skos:prefLabel "Museum of New Zealand Te Papa Tongarewa"@en ;
    skos:topConceptOf cs: ;
    schema:name "Museum of New Zealand Te Papa Tongarewa" ;
    schema:url "https://www.tepapa.govt.nz"^^xsd:anyURI ;
.

<https://linked.data.gov.au/org/tern>
    a
        skos:Concept ,
        schema:Organisation ;
    skos:definition "Terrestrial Ecosystems Research Network"@en ;
    skos:historyNote "From AGLDWG Orgs Catalogue https://catalogue.linked.data.gov.au/index.php/org/tern" ;
    skos:inScheme cs: ;
    skos:prefLabel "Terrestrial Ecosystems Research Network"@en ;
    skos:topConceptOf cs: ;
    schema:description "Australia’s land ecosystem observatory." ;
    schema:name "Terrestrial Ecosystems Research Network" ;
    schema:url "https://tern.org.au"^^xsd:anyURI ;
.

<https://linked.data.gov.au/org/tmag>
    a
        skos:Concept ,
        schema:Organization ;
    skos:definition """Tasmanian Museum and Art Gallery (TMAG) is Tasmania's leading natural and cultural heritage organisation. It is a combined museum, art gallery and herbarium which safeguards the physical evidence of Tasmania's natural and cultural heritage, and the cultural identity of Tasmanians.

TMAG is Australia's second-oldest museum and has its origins in the collections of Australia's oldest scientific society, the Royal Society of Tasmania, established in 1843.  The first permanent home of the museum opened on the corner of Argyle and Macquarie streets in 1863 and the museum has gradually expanded from this corner to occupy the entire city block."""@en ;
    skos:inScheme cs: ;
    skos:notation "17 334 217 592"^^<http://id.loc.gov/vocabulary/identifiers/ausbn> ;
    skos:prefLabel "Tasmanian Museum and Art Gallery"@en ;
    skos:topConceptOf cs: ;
    schema:name "Tasmanian Museum and Art Gallery" ;
    schema:url "https://www.tmag.tas.gov.au"^^xsd:anyURI ;
.

<https://linked.data.gov.au/org/uadelaide>
    a
        skos:Concept ,
        schema:Organization ;
    skos:definition "The University of Adelaide is a public research university based in Adelaide, South Australia. Established in 1874, it is the third-oldest university in Australia."@en ;
    skos:inScheme cs: ;
    skos:notation "61 249 878 937"^^<http://id.loc.gov/vocabulary/identifiers/ausbn> ;
    skos:prefLabel "University of Adelaide"@en ;
    skos:topConceptOf cs: ;
    schema:name "University of Adelaide" ;
    schema:url "https://www.adelaide.edu.au"^^xsd:anyURI ;
.

<https://linked.data.gov.au/org/umweltaust>
    a
        skos:Concept ,
        schema:Organization ;
    skos:definition "An employee-owned environmental and social professional services consultancy"@en ;
    skos:inScheme cs: ;
    skos:notation "18 059 519 041"^^<http://id.loc.gov/vocabulary/identifiers/ausbn> ;
    skos:prefLabel "Umwelt Australia Pty Ltd"@en ;
    skos:topConceptOf cs: ;
    schema:name "Umwelt Australia Pty Ltd" ;
    schema:url "https://www.umwelt.com.au"^^xsd:anyURI ;
.

<https://linked.data.gov.au/org/une>
    a
        skos:Concept ,
        schema:Organization ;
    skos:definition "The University of New England (UNE) is a public university in the New England region of the state of New South Wales, Australia. Founded in 1938, it was the first Australian university to be established outside of a state capital."@en ;
    skos:inScheme cs: ;
    skos:notation "75 792 454 315"^^<http://id.loc.gov/vocabulary/identifiers/ausbn> ;
    skos:prefLabel "University of New England"@en ;
    skos:topConceptOf cs: ;
    schema:name "University of New England" ;
    schema:url "https://www.une.edu.au"^^xsd:anyURI ;
.

<https://linked.data.gov.au/org/unsw>
    a
        skos:Concept ,
        schema:Organization ;
    skos:definition "The University of New South Wales (UNSW) is a public research university based in Sydney, New South Wales, Australia. It is one of the founding members of Group of Eight, a coalition of Australian research-intensive universities."@en ;
    skos:inScheme cs: ;
    skos:notation "57 195 873 179"^^<http://id.loc.gov/vocabulary/identifiers/ausbn> ;
    skos:prefLabel "The University of NSW"@en ;
    skos:topConceptOf cs: ;
    schema:name "The University of NSW" ;
    schema:url "https://www.unsw.edu.au"^^xsd:anyURI ;
.

<https://linked.data.gov.au/org/uom>
    a
        skos:Concept ,
        schema:Organization ;
    skos:definition "The University of Melbourne is a public research university located in Melbourne, Australia. Founded in 1853, it is Australia's second oldest university and the oldest in Victoria. Its main campus is located in Parkville, an inner suburb north of Melbourne's central business district, with several other campuses located across Victoria."@en ;
    skos:inScheme cs: ;
    skos:prefLabel "The University of Melbourne"@en ;
    skos:topConceptOf cs: ;
    schema:name "The University of Melbourne" ;
    schema:url "https://www.unimelb.edu.au"^^xsd:anyURI ;
.

<https://linked.data.gov.au/org/uq>
    a
        skos:Concept ,
        schema:Organization ;
    skos:definition "Ranked in the world's top 50, The University of Queensland is one of Australia's leading research and teaching institutions."@en ;
    skos:inScheme cs: ;
    skos:notation "63 942 912 684"^^<http://id.loc.gov/vocabulary/identifiers/ausbn> ;
    skos:prefLabel "University of Queensland"@en ;
    skos:topConceptOf cs: ;
    schema:name "University of Queensland" ;
    schema:url "https://www.uq.edu.au"^^xsd:anyURI ;
.

<https://linked.data.gov.au/org/vic-deeca>
    a
        skos:Concept ,
        schema:Organization ;
    skos:definition "DEECA brings together Victoria’s energy, environment, water, agriculture, forestry, resources, climate action, and emergency management functions into a single department to maximise connections between the environment, community, industry and economy."@en ;
    skos:inScheme cs: ;
    skos:prefLabel "Vic Department of Energy, Environment and Climate Action"@en ;
    skos:topConceptOf cs: ;
    schema:name "Vic Department of Energy, Environment and Climate Action" ;
    schema:url "https://www.deeca.vic.gov.au"^^xsd:anyURI ;
.

<https://linked.data.gov.au/org/wa-bio>
    a
        skos:Concept ,
        schema:Organization ;
    skos:definition "The Biodiversity Information Office (BIO) is responsible for making Western Australian biodiversity data more discoverable, accessible, and useable.  To deliver this change, BIO has developed the Dandjoo biodiversity data platform to mobilise data from all environment-related sectors, including government, industry, research, and the community.  BIO’s day-to-day work also includes a program of data-sharing and outreach work, identifying and sourcing priority datasets for release."@en ;
    skos:inScheme cs: ;
    skos:prefLabel "WA Biodiversity Information Office"@en ;
    skos:topConceptOf cs: ;
    schema:name "WA Biodiversity Information Office" ;
    schema:url "https://bio.wa.gov.au"^^xsd:anyURI ;
.

<https://linked.data.gov.au/org/wa-dbca>
    a
        skos:Concept ,
        schema:Organization ;
    skos:definition "The Department of Biodiversity, Conservation and Attractions (DBCA) is the Western Australian government department responsible for managing lands and waters described in the Conservation and Land Management Act 1984, the Rottnest Island Authority Act 1987, the Swan and Canning Rivers Management Act 2006, the Botanic Gardens and Parks Authority Act 1998, and the Zoological Parks Authority Act 2001, and implementing the state's conservation and environment legislation and regulations. The Department reports to the Minister for Environment and the Minister for Tourism. "@en ;
    skos:inScheme cs: ;
    skos:notation "38 052 249 024"^^<http://id.loc.gov/vocabulary/identifiers/ausbn> ;
    skos:prefLabel "WA Department of Biodiversity, Conservation and Attractions"@en ;
    skos:topConceptOf cs: ;
    schema:name "WA Department of Biodiversity, Conservation and Attractions" ;
    schema:url "https://www.dbca.wa.gov.au"^^xsd:anyURI ;
.

<https://linked.data.gov.au/org/wa-herbarium>
    a
        skos:Concept ,
        schema:Organization ;
    skos:definition "The Western Australian Herbarium is responsible for the description and documentation of Western Australia's exceptional botanical species diversity."@en ;
    skos:inScheme cs: ;
    skos:prefLabel "WA Herbarium"@en ;
    skos:topConceptOf cs: ;
    schema:name "WA Herbarium" ;
    schema:url "https://www.dbca.wa.gov.au/science/research-tools-and-repositories/western-australian-herbarium"^^xsd:anyURI ;
.

<https://linked.data.gov.au/org/wabsi>
    a
        skos:Concept ,
        schema:Organization ;
    skos:definition """A joint venture partnership with leading Western Australian science research organisations, with multi-disciplinary research expertise.

An independent, collaboration mechanism to facilitate end user driven, relevant biodiversity science research.

Funded by the Western Australian Government’s Department of Jobs, Tourism, Science and Innovation."""@en ;
    skos:inScheme cs: ;
    skos:prefLabel "Western Australian Biodiversity Science Institute"@en ;
    skos:topConceptOf cs: ;
    schema:name "Western Australian Biodiversity Science Institute" ;
    schema:url "https://wabsi.org.au"^^xsd:anyURI ;
.

<https://linked.data.gov.au/org/wam>
    a
        skos:Concept ,
        schema:Organization ;
    skos:definition """The Western Australian Museum is the State's premier cultural organisation, housing WA's scientific and cultural collection.

For over 120 years the Museum has been making the State's natural and social heritage accessible and engaging through research, exhibition and public programs.

Today, the Museum has seven public locations across the state - and a Collection and Research Centre that houses more than eight million objects."""@en ;
    skos:inScheme cs: ;
    skos:notation "95 249 517 733"^^<http://id.loc.gov/vocabulary/identifiers/ausbn> ;
    skos:prefLabel "Western Australian Museum"@en ;
    skos:topConceptOf cs: ;
    schema:name "Western Australian Museum" ;
    schema:url "https://visit.museum.wa.gov.au"^^xsd:anyURI ;
.

<https://linked.data.gov.au/org/western-shield>
    a
        skos:Concept ,
        schema:Organization ;
    skos:definition "WA’s largest conservation program, Western Shield, works to manage introduced predators for native species conservation. Learn what animals are protected, where DBCA’s fauna recovery sites are located, and what management tools are used. "@en ;
    skos:inScheme cs: ;
    skos:prefLabel "Western Shield"@en ;
    skos:topConceptOf cs: ;
    schema:name "Western Shield" ;
    schema:url "http://www.dbca.wa.gov.au/management/threat-management/invasive-animals/western-shield"^^xsd:anyURI ;
.

<https://linked.data.gov.au/org/wmbaustralia>
    a
        skos:Concept ,
        schema:Organization ;
    skos:definition "Acquired by BTM in 2008"@en ;
    skos:inScheme cs: ;
    skos:notation "54 010 830 421"^^<http://id.loc.gov/vocabulary/identifiers/ausbn> ;
    skos:prefLabel "WBM Oceanics Australia"@en ;
    skos:topConceptOf cs: ;
    schema:name "WBM Oceanics Australia" ;
    schema:url "https://www.bmt.org/services/environment-solutions"^^xsd:anyURI ;
.

<https://linked.data.gov.au/org/wwf-australia>
    a
        skos:Concept ,
        schema:Organization ;
    skos:definition "At WWF-Australia we’ve been protecting nature’s wonders for more than 40 years. And now we’re working with communities, governments, companies and others not just to protect our natural world but to restore and regenerate it."@en ;
    skos:inScheme cs: ;
    skos:notation "57 001 594 074"^^<http://id.loc.gov/vocabulary/identifiers/ausbn> ;
    skos:prefLabel "WWF Australia"@en ;
    skos:topConceptOf cs: ;
    schema:name "WWF Australia" ;
    schema:url "https://wwf.org.au"^^xsd:anyURI ;
.

cs:
    a skos:ConceptScheme ;
    skos:definition "Organisations known to own & submit data to the Biodiversity Date Repository"@en ;
    skos:hasTopConcept
        <https://linked.data.gov.au/org/act> ,
        <https://linked.data.gov.au/org/act-atlas> ,
        <https://linked.data.gov.au/org/am> ,
        <https://linked.data.gov.au/org/ambseh> ,
        <https://linked.data.gov.au/org/amnh> ,
        <https://linked.data.gov.au/org/ath> ,
        <https://linked.data.gov.au/org/awc> ,
        <https://linked.data.gov.au/org/awmm> ,
        <https://linked.data.gov.au/org/baam> ,
        <https://linked.data.gov.au/org/bdbsa> ,
        <https://linked.data.gov.au/org/bhp> ,
        <https://linked.data.gov.au/org/biepa> ,
        <https://linked.data.gov.au/org/birdlife> ,
        <https://linked.data.gov.au/org/canbr> ,
        <https://linked.data.gov.au/org/cooloolacc> ,
        <https://linked.data.gov.au/org/csiro> ,
        <https://linked.data.gov.au/org/dafwa> ,
        <https://linked.data.gov.au/org/des> ,
        <https://linked.data.gov.au/org/ecosmartecology> ,
        <https://linked.data.gov.au/org/gaia-resources> ,
        <https://linked.data.gov.au/org/gccc> ,
        <https://linked.data.gov.au/org/jcu> ,
        <https://linked.data.gov.au/org/latrobe> ,
        <https://linked.data.gov.au/org/lcai> ,
        <https://linked.data.gov.au/org/macleaymuseum> ,
        <https://linked.data.gov.au/org/mboca> ,
        <https://linked.data.gov.au/org/mgrt> ,
        <https://linked.data.gov.au/org/mjdenv> ,
        <https://linked.data.gov.au/org/mrcca> ,
        <https://linked.data.gov.au/org/museumsvictoria> ,
        <https://linked.data.gov.au/org/mwlr> ,
        <https://linked.data.gov.au/org/naturemapr> ,
        <https://linked.data.gov.au/org/nhm> ,
        <https://linked.data.gov.au/org/npansw> ,
        <https://linked.data.gov.au/org/nsw-bionet> ,
        <https://linked.data.gov.au/org/nsw-daff> ,
        <https://linked.data.gov.au/org/nsw-dcceew> ,
        <https://linked.data.gov.au/org/nsw-dpe> ,
        <https://linked.data.gov.au/org/nsw-dpie> ,
        <https://linked.data.gov.au/org/nsw-npws> ,
        <https://linked.data.gov.au/org/nt-atlas> ,
        <https://linked.data.gov.au/org/nt-dipe> ,
        <https://linked.data.gov.au/org/nt-dlpe> ,
        <https://linked.data.gov.au/org/nt-dlrm> ,
        <https://linked.data.gov.au/org/nt-herbarium> ,
        <https://linked.data.gov.au/org/qld-daff> ,
        <https://linked.data.gov.au/org/qld-derm> ,
        <https://linked.data.gov.au/org/qld-detsi> ,
        <https://linked.data.gov.au/org/qld-dres> ,
        <https://linked.data.gov.au/org/qld-tmr> ,
        <https://linked.data.gov.au/org/qld-tsgehp> ,
        <https://linked.data.gov.au/org/qld-wildnet> ,
        <https://linked.data.gov.au/org/qm> ,
        <https://linked.data.gov.au/org/qnc> ,
        <https://linked.data.gov.au/org/qpws> ,
        <https://linked.data.gov.au/org/qvmag> ,
        <https://linked.data.gov.au/org/rbgdt> ,
        <https://linked.data.gov.au/org/rbgv> ,
        <https://linked.data.gov.au/org/reefcatchments> ,
        <https://linked.data.gov.au/org/riotinto> ,
        <https://linked.data.gov.au/org/sa-dew> ,
        <https://linked.data.gov.au/org/sa-dewnr> ,
        <https://linked.data.gov.au/org/sa-herbarium> ,
        <https://linked.data.gov.au/org/sam> ,
        <https://linked.data.gov.au/org/scienceforwildlife> ,
        <https://linked.data.gov.au/org/scion> ,
        <https://linked.data.gov.au/org/sfsgi> ,
        <https://linked.data.gov.au/org/sunwater> ,
        <https://linked.data.gov.au/org/te-papa> ,
        <https://linked.data.gov.au/org/tern> ,
        <https://linked.data.gov.au/org/tmag> ,
        <https://linked.data.gov.au/org/uadelaide> ,
        <https://linked.data.gov.au/org/umweltaust> ,
        <https://linked.data.gov.au/org/une> ,
        <https://linked.data.gov.au/org/unsw> ,
        <https://linked.data.gov.au/org/uom> ,
        <https://linked.data.gov.au/org/uq> ,
        <https://linked.data.gov.au/org/vic-deeca> ,
        <https://linked.data.gov.au/org/wa-bio> ,
        <https://linked.data.gov.au/org/wa-dbca> ,
        <https://linked.data.gov.au/org/wa-herbarium> ,
        <https://linked.data.gov.au/org/wabsi> ,
        <https://linked.data.gov.au/org/wam> ,
        <https://linked.data.gov.au/org/western-shield> ,
        <https://linked.data.gov.au/org/wmbaustralia> ,
        <https://linked.data.gov.au/org/wwf-australia> ;
    skos:historyNote
        """2025-08: Added from data supplied to the BDR from jurisdictions via https://submit.bdr.gov.au in mid-2025" ,

This vocabulary was initially developed for the Biodiversity Data Repository and is live in that it grows with new data submissions from new organisations""" ,
        "Added from data supplied to tne BDR from jurisdictions via https://submit.bdr.gov.au in mid-2025" ,
        "This vocabulary was developed for the Biodiversity Data Repository and is live in that it grows with new data submissions from new organisations" ;
    skos:prefLabel "BDR Organisations"@en ;
    schema:creator <https://linked.data.gov.au/org/dcceew> ;
    schema:dateCreated "2024-07-09"^^xsd:date ;
    schema:dateModified "2025-08-19"^^xsd:date ;
    schema:license <http://purl.org/NET/rdflicense/cc-by4.0> ;
    schema:publisher <https://linked.data.gov.au/org/dcceew> ;
.
