PREFIX : <https://linked.data.gov.au/dataset/bdr/sma/>
PREFIX cs: <https://linked.data.gov.au/dataset/bdr/sma>
PREFIX schema: <https://schema.org/>
PREFIX skos: <http://www.w3.org/2004/02/skos/core#>
PREFIX xsd: <http://www.w3.org/2001/XMLSchema#>


:Insert
    a skos:Concept ;
    skos:definition "Insert submission into the BDR Graph. This is used for the delivery of new Datasets, new BDR Sites, new Systematic-Survey submissions, and new Incidential Occurrences."@en ;
    skos:historyNote "Defined by the BDR Team for use in data submissions to the BDR" ;
    skos:scopeNote "In the BDR Data Ingestion pipeline, the submission must pass validation before it is inserted.";
    skos:inScheme cs: ;
    skos:prefLabel "Insert"@en ;
    skos:topConceptOf cs: ;
.

:Update
    a skos:Concept ;
    skos:definition "Validate the RDF data associated with the submission then use it as a delta to update existing data in the BDR Graph. This is used for updating Dataset metadata, modifying existing Sites, and modifying existing Systematic-Survey submissions."@en ;
    skos:historyNote "Defined by the BDR Team for use in data submissions to the BDR" ;
    skos:scopeNote "Updating an entity that does not exist will return an error. In the BDR Data Ingestion pipeline, the delta submission must pass validation before it is used to update the dataset." ;
    skos:inScheme cs: ;
    skos:prefLabel "Update"@en ;
    skos:topConceptOf cs: ;
.

:Remove
    a skos:Concept ;
    skos:definition "Remove the associated RDF assets from the BDR Graph. This is used for removal of Dataset metadata, removal of Incidental Occurrences from a Dataset, and removal of entities within a Systematic-Survey."@en ;
    skos:scopeNote "This action cannot be used to remove a complete BDR Dataset. Email the BDR team discuss the complete remove of a Dataset." ;
    skos:historyNote "Defined by the BDR Team for use in data submissions to the BDR" ;
    skos:inScheme cs: ;
    skos:prefLabel "Remove"@en ;
    skos:topConceptOf cs: ;
.

:Check
    a skos:Concept ;
    skos:definition "Only validate the submission, and do not insert it into the BDR Graph."@en ;
    skos:historyNote "Defined by the BDR Team for use in testing data submissions to the BDR" ;
    skos:scopeNote "This is the same as Insert but it does not ingest the resulting subgraph to the BDR.";
    skos:inScheme cs: ;
    skos:prefLabel "Check"@en ;
    skos:topConceptOf cs: ;
.

cs:
    a skos:ConceptScheme ;
    skos:definition "Collection of actions for a Submission Manifest that provide hints for how to process a BDR Submissions"@en ;
    skos:historyNote "This vocabulary was developed to assist with the processing of submissions and updates to the Biodiversity Data Repository in March 2025" ;
    skos:prefLabel "BDR Submission Manifest Actions"@en ;
    skos:scopeNote "See the ABIS Specification, <https://linked.data.gov.au/def/abis> - BDR Profile Section, for the definition of BDR Submission Manifest Actions"@en ;
    schema:creator <https://linked.data.gov.au/org/dcceew> ;
    schema:dateCreated "2025-03-18"^^xsd:date ;
    schema:dateModified "2025-03-18"^^xsd:date ;
    schema:license <http://purl.org/NET/rdflicense/cc-by4.0> ;
    schema:publisher <https://linked.data.gov.au/org/dcceew> ;
    skos:hasTopConcept 
        :Insert ,
        :Update ,
        :Remove ,
        :Check ;
.
