PREFIX : <https://linked.data.gov.au/dataset/bdr/statsprops/>
PREFIX cs: <https://linked.data.gov.au/dataset/bdr/statsprops>
PREFIX owl: <http://www.w3.org/2002/07/owl#>
PREFIX schema: <https://schema.org/>
PREFIX skos: <http://www.w3.org/2004/02/skos/core#>
PREFIX sosa: <http://www.w3.org/ns/sosa/>
PREFIX xsd: <http://www.w3.org/2001/XMLSchema#>


:DataStatistic
    a skos:Concept , sosa:ObservableProperty ;
    skos:definition "A statistic of data within a given scope"@en ;
    skos:historyNote "Defined by BDR admin" ;
    skos:inScheme cs: ;
    skos:prefLabel "Data Statistic"@en ;
    skos:topConceptOf cs: ;
.

:ObservationsCount
    a skos:Concept , sosa:ObservableProperty ;
    skos:definition "The number of ABIS Observation class instances within a given scope"@en ;
    skos:historyNote "Defined by BDR admin" ;
    skos:inScheme cs: ;
    skos:prefLabel "Observations Count"@en ;
    skos:broader :DataStatistic ;
.

:SamplesCount
    a skos:Concept , sosa:ObservableProperty ;
    skos:definition "The number of SOSA Sample class instances within a given scope"@en ;
    skos:historyNote "Defined by BDR admin" ;
    skos:inScheme cs: ;
    skos:prefLabel "Samples Count"@en ;
    skos:broader :DataStatistic ;
.

:SamplingsCount
    a skos:Concept , sosa:ObservableProperty ;
    skos:definition "The number of SOSA Sampling class instances within a given scope"@en ;
    skos:historyNote "Defined by BDR admin" ;
    skos:inScheme cs: ;
    skos:prefLabel "Samplings Count"@en ;
    skos:broader :DataStatistic ;
.

:OccurrencesCount
    a skos:Concept , sosa:ObservableProperty ;
    skos:definition "The number of ABIS Occurrence class instances within a given scope"@en ;
    skos:historyNote "Defined by BDR admin" ;
    skos:inScheme cs: ;
    skos:prefLabel "Occurrences Count"@en ;
    skos:broader :DataStatistic ;
.

:SubmissionCount
    a skos:Concept , sosa:ObservableProperty ;
    skos:definition "The number of ABIS Submission (tern:RDFDataset) class instances within a given scope"@en ;
    skos:historyNote "Defined by BDR admin" ;
    skos:inScheme cs: ;
    skos:prefLabel "Submission Count"@en ;
    skos:broader :DataStatistic ;
.

:BiodiversityRecordsCount
    a skos:Concept , sosa:ObservableProperty ;
    skos:definition "The number of ABIS Biodiversity Records class instances within a given scope"@en ;
    skos:historyNote "Defined by BDR admin" ;
    skos:inScheme cs: ;
    skos:prefLabel "BiodiversityRecords Count"@en ;
    skos:broader :DataStatistic ;
.

:SiteCount
    a skos:Concept , sosa:ObservableProperty ;
    skos:definition "The number of TERN Site class instances within a given scope"@en ;
    skos:historyNote "Defined by BDR admin" ;
    skos:inScheme cs: ;
    skos:prefLabel "Site Count"@en ;
    skos:broader :DataStatistic ;
.

:SiteVisitCount
    a skos:Concept , sosa:ObservableProperty ;
    skos:definition "The number of TERN SiteVisit class instances within a given scope"@en ;
    skos:historyNote "Defined by BDR admin" ;
    skos:inScheme cs: ;
    skos:prefLabel "SiteVisit Count"@en ;
    skos:broader :DataStatistic ;
.

:SurveyCount
    a skos:Concept , sosa:ObservableProperty ;
    skos:definition "The number of TERN Survey class instances within a given scope"@en ;
    skos:historyNote "Defined by BDR admin" ;
    skos:inScheme cs: ;
    skos:prefLabel "Survey Count"@en ;
    skos:broader :DataStatistic ;
.

:DatasetsCount
    a skos:Concept , sosa:ObservableProperty ;
    skos:definition "The number of ABIS Dataset (schema:Dataset) class instances within a given scope"@en ;
    skos:historyNote "Defined by BDR admin" ;
    skos:inScheme cs: ;
    skos:prefLabel "Datasets Count"@en ;
    skos:broader :DataStatistic ;
.


cs:
    a skos:ConceptScheme ;
    skos:definition """Statistical Properties - These are observable properties that describe statistics of BDR Datasets."""@en ;
    skos:hasTopConcept :DataStatistic ;
    skos:historyNote "This vocabulary was developed for the Biodiversity Data Repository as a catch-all vocab/register of observable properties which are not characterised elsewhere" ;
    skos:prefLabel "BDR Observable Properties"@en ;
    schema:creator <https://linked.data.gov.au/org/dcceew> ;
    schema:dateCreated "2024-07-10"^^xsd:date ;
    schema:dateModified "2024-07-10"^^xsd:date ;
    schema:license <http://purl.org/NET/rdflicense/cc-by4.0> ;
    schema:publisher <https://linked.data.gov.au/org/dcceew> ;
.
