PREFIX : <https://linked.data.gov.au/dataset/bdr/smrr/>
PREFIX cs: <https://linked.data.gov.au/dataset/bdr/submission_actions>
PREFIX schema: <https://schema.org/>
PREFIX skos: <http://www.w3.org/2004/02/skos/core#>
PREFIX xsd: <http://www.w3.org/2001/XMLSchema#>


:ValidateAndInsert
    a skos:Concept ;
    skos:definition "Validate the RDF data associated with the submission then insert it into the BDR Graph. This is used for the delivery of new Datasets, new BDR Sites, new Systematic-Survey submissions, and new Incidential Occurrences."@en ;
    skos:historyNote "Defined by the BDR Team for use in data submissions to the BDR" ;
    skos:inScheme cs: ;
    skos:prefLabel "Validate And Insert"@en ;
    skos:topConceptOf cs: ;
.


:ValidateAndUpdate
    a skos:Concept ;
    skos:definition "Validate the RDF data associated with the submission then use it as a delta to update existing data in the BDR Graph. This is used for updating Dataset metadata, modifying existing Sites, and modifying existing Systematic-Survey submissions."@en ;
    skos:historyNote "Defined by the BDR Team for use in data submissions to the BDR" ;
    skos:inScheme cs: ;
    skos:prefLabel "Validate And Update"@en ;
    skos:topConceptOf cs: ;
.

:Remove
    a skos:Concept ;
    skos:definition "Remove the associated RDF assets from the BDR Graph. This is used for removal of Dataset metadata, removal of Incidental Occurrences from a Dataset, and removal of entities within a Systematic-Survey."@en ;
    skos:scopeNote "This action cannot be used to remove a complete BDR Dataset. Email the BDR team discuss the complete remove of a Dataset." ;
    skos:historyNote "Defined by the BDR Team for use in data submissions to the BDR" ;
    skos:inScheme cs: ;
    skos:prefLabel "Remove"@en ;
    skos:topConceptOf cs: ;
.

cs:
    a skos:ConceptScheme ;
    skos:definition "Collection of actions for a Submission Manifest that provide hints for how to process a BDR Submissions"@en ;
    skos:historyNote "This vocabulary was developed to assist with the processing of submissions and updates to the Biodiversity Data Repository in March 2025" ;
    skos:prefLabel "BDR Submission Manifest Actions"@en ;
    skos:scopeNote "See the ABIS Specification, <https://linked.data.gov.au/def/abis> - BDR Profile Section, for the definition of BDR Submission Manifest Actions"@en ;
    schema:creator <https://linked.data.gov.au/org/dcceew> ;
    schema:dateCreated "2025-03-13"^^xsd:date ;
    schema:dateModified "2025-03-13"^^xsd:date ;
    schema:license <http://purl.org/NET/rdflicense/cc-by4.0> ;
    schema:publisher <https://linked.data.gov.au/org/dcceew> ;
    skos:hasTopConcept 
        :ValidateAndInsert ,
        :ValidateAndUpdate ,
        :Remove ;
.
